proof for TestSuffix

verif/trie/representation/key.v
@@ -1,4 +1,6 @@
 (** * bordernode_rep.v : Formalization for representation relationship of bordernode *)
+Require Import VST.floyd.proofauto.
+Require Import VST.floyd.library.
 Require Import deepDB.common.
 
 (* seplog part *)
@@ -10,17 +12,16 @@ Require Import deepDB.prog.
 Definition tkey: type := Tstruct _KVKey noattr.
 Definition tkeybox: type := tptr tkey.
 
-Definition key_rep (sh: share) (key: string) (p: val) :=
-  EX p':val,
+Definition key_rep (sh: share) (key: string) (p: val) (p':val) :=
   data_at sh tkey (p', Vint (Int.repr (Zlength key))) p *
+  malloc_token Tsh (tarray tschar (Zlength key)) p' *
   cstring_len Tsh key p'.
 
 Lemma keyrep_fold (sh: share) (key: string) (p: val) (p': val):
-  data_at sh tkey (p', Vint (Int.repr (Zlength key))) p * cstring_len Tsh key p' |--
-  key_rep sh key p.
+  data_at sh tkey (p', Vint (Int.repr (Zlength key))) p * malloc_token Tsh (tarray tschar (Zlength key)) p' * cstring_len Tsh key p' |--
+  key_rep sh key p p'.
 Proof.
   unfold key_rep.
-  Exists p'.
   cancel.
 Qed.
 
@@ -30,14 +31,18 @@ Ltac fold_keyrep :=
   | |- context [data_at ?sh tkey (?p', Vint (Int.repr ?len)) ?p] =>
     match goal with
     | |- context [cstring_len Tsh ?key p'] =>
-      replace len with (Zlength key) by list_solve;
-      sep_apply (keyrep_fold sh key p p')
+      match goal with
+      | |- context [malloc_token Tsh (tarray tschar ?len') p'] =>
+        replace len with (Zlength key) by list_solve;
+        replace len' with (Zlength key) by list_solve;
+        sep_apply (keyrep_fold sh key p p')
+      end
     end
   end.
 
 Lemma fold_keyrep_example (sh: share) (key1 key2: string) (p: val) (p': val):
   0 < Zlength key1 + Zlength key2 <= Int.max_unsigned ->
-  data_at sh tkey (p', Vint (Int.repr (Zlength key1 + Zlength key2))) p * data_at Tsh (tarray tschar (Zlength (key1 ++ key2))) (map Vbyte key1 ++ map Vbyte key2) p' |-- key_rep sh (key1 ++ key2) p.
+  data_at sh tkey (p', Vint (Int.repr (Zlength key1 + Zlength key2))) p * data_at Tsh (tarray tschar (Zlength (key1 ++ key2))) (map Vbyte key1 ++ map Vbyte key2) p' * malloc_token Tsh (tarray tschar (Zlength key1 + Zlength key2)) p' |-- key_rep sh (key1 ++ key2) p p'.
 Proof.
   intros.
   rewrite <- map_app.
