verif/trie/prog.v
@@ -1,0 +1,5 @@
+Require Export VST.floyd.proofauto.
+Require Export deepDB.clight.verifiable.
+
+Instance CompSpecs : compspecs. make_compspecs prog. Defined.
+Definition Vprog : varspecs. mk_varspecs prog. Defined.
